Models.v
@@ -5,7 +5,7 @@
     This file is released under the CC0 License, see the LICENSE file *)
 
 Require Import Eqdep_dec Defs Mix NameProofs Meta.
-Require Import Theories NaryFunctions Nary PreModels.
+Require Import Wellformed Theories NaryFunctions Nary PreModels.
 Import ListNotations.
 Local Open Scope bool_scope.
 Local Open Scope lazy_bool_scope.
@@ -23,7 +23,7 @@ Lemma validity_theorem logic th :
 Proof.
  intros CR T Thm M mo genv.
  rewrite thm_alt in Thm.
- destruct Thm as (WF & d & axs & (CK & BC & V) & F & C).
+ destruct Thm as (WF & d & axs & ((CK & BC) & V) & F & C).
  assert (CO:=@correctness th M mo logic d CR V BC genv).
  rewrite C in CO. apply CO. intros A HA. apply AxOk.
  rewrite Forall_forall in F; auto.
@@ -37,113 +37,17 @@ Proof.
  apply (validity_theorem _ _ CR _ Thm M mo (fun _ => mo.(someone))).
 Qed.
 
-Lemma Thm_Not_e th A :
- IsTheorem Classic th A -> IsTheorem Classic th (~A) ->
- IsTheorem Classic th False.
-Proof.
- intros (_ & axs & F & PR) (_ & axs' & F' & PR').
- split. apply False_wf.
- exists (axs++axs'); split.
- rewrite Forall_forall in *; intros x; rewrite in_app_iff;
-  intros [ | ]; auto.
- apply R_Not_e with A.
- - clear PR'; eapply Pr_weakening; eauto. constructor.
-   intros a. rewrite in_app_iff; auto.
- - eapply Pr_weakening; eauto. constructor.
-   intros a. rewrite in_app_iff; auto.
-Qed.
 
-Definition Wf_term (sign:signature) (t:term) :=
-  check sign t = true /\ BClosed t /\ FClosed t.
+Definition wcterm sign :=
+ { t : term | wc sign t = true }.
 
-Definition wf_term (sign:signature) (t:term) :=
- check sign t && (level t =? 0) && Names.is_empty (fvars t).
-
-Lemma Wf_term_alt sign t : Wf_term sign t <-> wf_term sign t = true.
-Proof.
- unfold Wf_term, wf_term.
- split.
- - intros (-> & -> & H). cbn. now rewrite Names.is_empty_spec.
- - rewrite !andb_true_iff, !eqb_eq. unfold BClosed.
-   intros ((->,->),H); repeat split; auto.
-   now rewrite Names.is_empty_spec in H.
-Qed.
-
-Lemma Fun_wf sign f l :
-  Wf_term sign (Fun f l) <->
-   sign.(funsymbs) f = Some (length l) /\ Forall (Wf_term sign) l.
-Proof.
- split.
- - intros (CK & BC & FC); cbn in *.
-   destruct (funsymbs _ f); [|easy].
-   rewrite lazy_andb_iff, eqb_eq in CK.
-   destruct CK as (->,CK). split; auto.
-   rewrite forallb_forall in CK.
-   apply Forall_forall. intros t Ht.
-   repeat split; auto.
-   + unfold BClosed in *. cbn in BC.
-     rewrite list_max_map_0 in BC; auto.
-   + unfold FClosed in *. cbn in FC.
-     intros v. eapply unionmap_notin; eauto.
- - intros (E,F).
-   rewrite Forall_forall in F.
-   repeat split; cbn.
-   + rewrite E, eqb_refl. apply forallb_forall.
-     intros u Hu. now apply F.
-   + red; cbn. apply list_max_map_0. intros u Hu. now apply F.
-   + red; cbn. intro v. rewrite unionmap_in.
-     intros (a & IN & IN'). apply F in IN'. now apply IN' in IN.
-Qed.
-
-Lemma Pred_wf sign p l :
-  Wf sign (Pred p l) <->
-   sign.(predsymbs) p = Some (length l) /\ Forall (Wf_term sign) l.
-Proof.
- split.
- - intros (CK & BC & FC); cbn in *.
-   destruct (predsymbs _ p); [|easy].
-   rewrite lazy_andb_iff, eqb_eq in CK.
-   destruct CK as (->,CK). split; auto.
-   rewrite forallb_forall in CK.
-   apply Forall_forall. intros t Ht.
-   repeat split; auto.
-   + unfold BClosed in *. cbn in BC.
-     rewrite list_max_map_0 in BC; auto.
-   + unfold FClosed in *. cbn in FC.
-     intros v. eapply unionmap_notin; eauto.
- - intros (E,F).
-   rewrite Forall_forall in F.
-   repeat split; cbn.
-   + rewrite E, eqb_refl. apply forallb_forall.
-     intros u Hu. now apply F.
-   + red; cbn. apply list_max_map_0. intros u Hu. now apply F.
-   + red; cbn. intro v. rewrite unionmap_in.
-     intros (a & IN & IN'). apply F in IN'. now apply IN' in IN.
-Qed.
-
-Lemma Cst_wf sign c :
-  sign.(funsymbs) c = Some 0 -> Wf_term sign (Cst c).
-Proof.
- intros. now apply Fun_wf.
-Qed.
-
-Lemma Cst_wf' sign c :
-  sign.(funsymbs) c = Some 0 -> wf_term sign (Cst c) = true.
-Proof.
- intros. now apply Wf_term_alt, Fun_wf.
-Qed.
-
-
-Definition closed_term sign :=
- { t : term | wf_term sign t = true }.
-
-Lemma proof_irr sign (s s' : closed_term sign) :
+Lemma proof_irr sign (s s' : wcterm sign) :
  s = s' <-> proj1_sig s = proj1_sig s'.
 Proof.
  destruct s, s'. cbn. split.
  - now injection 1.
  - intros <-. f_equal.
-   destruct (wf_term sign x); [|easy].
+   destruct (wc sign x); [|easy].
    rewrite UIP_refl_bool. apply UIP_refl_bool.
 Qed.
 
@@ -153,40 +57,40 @@ Variable th : theory.
 Variable oneconst : string.
 Hypothesis Honeconst : th.(funsymbs) oneconst = Some 0.
 
-Let M := closed_term th.
+Let M := wcterm th.
 
 Lemma cons_ok (t : term) (l : list term) n :
- wf_term th t = true ->
- length l = n /\ Forall (Wf_term th) l ->
- length (t::l) = S n /\ Forall (Wf_term th) (t::l).
+ wc th t = true ->
+ length l = n /\ Forall (WC th) l ->
+ length (t::l) = S n /\ Forall (WC th) (t::l).
 Proof.
  intros WF (L,F).
- apply Wf_term_alt in WF.
+ apply term_wc_iff in WF.
  split; simpl; auto.
 Qed.
 
-Definition sized_wf_listterm n :=
-  {l : list term | length l = n /\ Forall (Wf_term th) l}.
+Definition sized_wc_listterm n :=
+  {l : list term | length l = n /\ Forall (WC th) l}.
 
-Fixpoint mk_args n : M^^n --> sized_wf_listterm n :=
+Fixpoint mk_args n : M^^n --> sized_wc_listterm n :=
  match n with
  | 0 => exist _ [] (conj eq_refl (Forall_nil _))
  | S n => fun t =>
-          map_arity (fun '(exist _ l Hl) =>
+          nfun_to_nfun (fun '(exist _ l Hl) =>
                        let '(exist _ t Ht) := t in
                        exist _ (t::l) (cons_ok t l n Ht Hl))
                     (mk_args n)
  end.
 
-Definition one_listterm n : sized_wf_listterm n.
+Definition one_listterm n : sized_wc_listterm n.
 Proof.
  induction n as [|n (l & L & F)].
  - now exists [].
  - exists (Cst oneconst :: l).
-   split; simpl; auto using Cst_wf.
+   split; simpl; auto using Cst_WC.
 Qed.
 
-Lemma build_mk n (l : list M) (any:sized_wf_listterm n) :
+Lemma build_mk n (l : list M) (any:sized_wc_listterm n) :
  length l = n ->
  proj1_sig (build_args l any (mk_args n)) =
  map (@proj1_sig _ _) l.
@@ -194,7 +98,7 @@ Proof.
  intros <-.
  induction l as [|(t,Ht) l IH]; simpl; auto.
  set (l0 := one_listterm (length l)).
- rewrite build_map_arity  with (any0:=l0); auto.
+ rewrite build_args_ntn  with (any0:=l0); auto.
  specialize (IH l0).
  destruct (build_args _); simpl in *. f_equal; auto.
 Qed.
@@ -204,8 +108,8 @@ Definition fun_core f n :
 Proof.
  intros E.
  generalize (mk_args n).
- apply map_arity. intros (l & Hl).
- exists (Fun f l). apply Wf_term_alt, Fun_wf; destruct Hl; subst; auto.
+ apply nfun_to_nfun. intros (l & Hl).
+ exists (Fun f l). apply term_wc_iff, Fun_WC; destruct Hl; subst; auto.
 Defined.
 
 Definition rich_funs f :
@@ -224,7 +128,7 @@ Proof.
    exists (NFun _ r); split; auto.
    intros l any Hl.
    unfold r, fun_core.
-   rewrite build_map_arity with (any0 := one_listterm n); auto.
+   rewrite build_args_ntn with (any0 := one_listterm n); auto.
    rewrite <- (build_mk n l (one_listterm n) Hl).
    destruct build_args. now cbn.
  - now exists Nop.
@@ -244,7 +148,7 @@ Proof.
  destruct (th.(predsymbs) p) as [n|].
  - apply (NFun n).
    generalize (mk_args n).
-   apply map_arity.
+   apply nfun_to_nfun.
    exact (fun sl => IsTheorem logic th (Pred p (proj1_sig sl))).
  - apply Nop.
 Defined.
@@ -256,7 +160,7 @@ Proof.
 Qed.
 
 Definition SyntacticPreModel : PreModel M th :=
- {| someone := exist _ (Cst oneconst) (Cst_wf' _ _ Honeconst);
+ {| someone := exist _ (Cst oneconst) (Cst_wc _ _ Honeconst);
     funs := mk_funs;
     preds := mk_preds;
     funsOk := mk_funs_ok;
@@ -272,7 +176,7 @@ Hypothesis witsat : WitnessSaturated Classic th.
 Variable oneconst : string.
 Hypothesis Honeconst : th.(funsymbs) oneconst = Some 0.
 
-Let M := closed_term th.
+Let M := wcterm th.
 Let mo : PreModel M th :=
  SyntacticPreModel Classic th oneconst Honeconst.
 
@@ -288,7 +192,7 @@ Proof.
  revert t.
  fix IH 1. destruct t as [ | | f l]; cbn; auto.
  - destruct (genv v) as (t,Ht); cbn; auto.
-   apply Wf_term_alt in Ht. apply Ht.
+   apply term_wc_iff in Ht. apply Ht.
  - rewrite map_length.
    destruct (funsymbs th f); [|easy].
    case eqb; [|easy].
@@ -302,28 +206,21 @@ Proof.
  revert t.
  fix IH 1. destruct t as [ | | f l]; cbn; auto.
  - destruct (genv v) as (t,Ht); cbn; auto.
-   apply Wf_term_alt in Ht. apply Ht.
+   apply term_wc_iff in Ht. apply Ht.
  - revert l. fix IH' 1. destruct l as [|t l]; cbn; auto.
    f_equal. apply IH. apply IH'.
-Qed.
-
-Lemma empty_union s s' : Names.Empty (Names.union s s') <->
- Names.Empty s /\ Names.Empty s'.
-Proof.
- split. split; namedec. namedec.
 Qed.
 
 Lemma term_closure_fclosed t (genv:variable->M) :
   FClosed (term_closure genv t).
 Proof.
- revert t.
- fix IH 1. destruct t as [ | | f l]; cbn; auto.
+ induction t using term_ind'; cbn; auto.
  - destruct (genv v) as (t,Ht); cbn; auto.
-   apply Wf_term_alt in Ht. apply Ht.
- - unfold FClosed in *. cbn.
-   revert l. fix IH' 1. destruct l as [|t l]; cbn; auto.
-   unfold term_closure in *.
-   apply empty_union; auto.
+   apply term_wc_iff in Ht. apply Ht.
+ - change (FClosed (Fun f (map (term_closure genv) args))).
+   rewrite <- term_fclosed_spec. cbn.
+   apply forallb_forall. intros a Ha. rewrite term_fclosed_spec.
+   rewrite in_map_iff in Ha. destruct Ha as (x & <- & IN); auto.
 Qed.
 
 Lemma closure_check f genv :
@@ -335,7 +232,6 @@ Proof.
    case eqb; [|easy].
    revert l.
    induction l as [|t l]; cbn; auto. f_equal; auto.
-   change (check th (term_closure genv t) = check th t). (* TODO *)
    apply term_closure_check.
  - unfold closure in *. now rewrite IHf1, IHf2.
 Qed.
@@ -353,36 +249,33 @@ Lemma closure_fclosed f (genv:variable->M) :
   FClosed (closure genv f).
 Proof.
  induction f; cbn; auto.
- - unfold FClosed in *. cbn.
-   revert l. induction l as [|t l IH]; cbn; auto.
-   apply empty_union; split; auto.
-   apply (term_closure_fclosed t genv).
- - unfold FClosed in *. cbn.
-   apply empty_union; split; auto.
+ - change (FClosed (Pred p (map (term_closure genv) l))).
+   rewrite <- form_fclosed_spec. cbn.
+   apply forallb_forall. intros a Ha. rewrite term_fclosed_spec.
+   rewrite in_map_iff in Ha.
+   destruct Ha as (x & <- & IN); auto using term_closure_fclosed.
+ - rewrite <- form_fclosed_spec in *. cbn. now rewrite lazy_andb_iff.
 Qed.
 
-Lemma term_closure_wf t genv :
-  check th t = true -> BClosed t ->
-  Wf_term th (term_closure genv t).
+Lemma term_closure_wc t genv :
+  WF th t -> WC th (term_closure genv t).
 Proof.
- repeat split.
+ intros (?,?). repeat split.
  - now rewrite term_closure_check.
  - red. now rewrite term_closure_level.
  - apply term_closure_fclosed.
 Qed.
 
-Lemma term_closure_wf' t genv :
-  check th t = true -> BClosed t ->
-  wf_term th (term_closure genv t) = true.
+Lemma term_closure_wc' t genv :
+  WF th t -> wc th (term_closure genv t) = true.
 Proof.
- intros CK BC. apply Wf_term_alt. now apply term_closure_wf.
+ intro. apply term_wc_iff. now apply term_closure_wc.
 Qed.
 
-Lemma closure_wf f genv :
-  check th f = true -> BClosed f ->
-  Wf th (closure genv f).
+Lemma closure_wc f genv :
+  WF th f -> WC th (closure genv f).
 Proof.
- repeat split.
+ intros (?,?). repeat split.
  - now rewrite closure_check.
  - red. now rewrite closure_level.
  - apply closure_fclosed.
@@ -399,37 +292,36 @@ Proof.
  rewrite term_vmap_id; auto.
  intros v. red in FC. intuition.
  intros v. destruct (genv v) as (u,Hu); simpl.
- apply Wf_term_alt in Hu. apply Hu.
+ apply term_wc_iff in Hu. apply Hu.
 Qed.
 
 Lemma interp_pred p l :
- check th (Pred p l) = true ->
- BClosed (Pred p l) ->
+ WF th (Pred p l) ->
  forall genv,
    interp_form mo genv [] (Pred p l) <->
    IsTheorem Classic th
      (Pred p (map (fun t => proj1_sig (interp_term mo genv [] t)) l)).
 Proof.
- unfold BClosed. cbn.
+ unfold WF, BClosed. cbn.
  destruct (predsymbs th p) as [n|] eqn:E; [|easy].
- rewrite lazy_andb_iff, eqb_eq. intros (L,CK) BC genv.
+ rewrite lazy_andb_iff, eqb_eq. intros ((L,CK),BC) genv.
  unfold mk_preds; rewrite E. cbn. clear E.
  set (l0 := one_listterm th oneconst Honeconst n).
- rewrite build_map_arity with (any := l0) by now rewrite map_length.
+ rewrite build_args_ntn with (any := l0) by now rewrite map_length.
  rewrite build_mk with (oneconst := oneconst) by (auto; now rewrite map_length).
  rewrite map_map; reflexivity.
 Qed.
 
 Lemma interp_term_carac t :
-  check th t = true -> BClosed t ->
+  WF th t ->
   forall genv,
     proj1_sig (interp_term mo genv [] t) = term_closure genv t.
 Proof.
  induction t as [ | | f l IH] using term_ind'; cbn; auto.
- - unfold BClosed. cbn. easy.
- - destruct (funsymbs th f) as [n|] eqn:E; [|easy].
+ - now unfold WF,BClosed.
+ - unfold WF. cbn. destruct (funsymbs th f) as [n|] eqn:E; [|easy].
    rewrite lazy_andb_iff, eqb_eq.
-   intros (L,CK) BC genv.
+   intros ((L,CK),BC) genv.
    unfold mk_funs.
    destruct rich_funs as ([n' a| ] & Ho & Ho'); cbn in *.
    2: congruence.
@@ -439,20 +331,19 @@ Proof.
    clear Ho Ho'.
    rewrite map_map.
    f_equal. apply map_ext_iff.
-   intros t Ht. apply IH; auto.
+   intros t Ht. apply IH; auto. split.
    + rewrite forallb_forall in CK; auto.
    + red in BC. cbn in BC. rewrite list_max_map_0 in BC; auto.
 Qed.
 
-Lemma interp_term_carac' (t:term) genv
-  (CK : check th t = true) (BC : BClosed t) :
+Lemma interp_term_carac' (t:term) genv (W : WF th t) :
   interp_term mo genv [] t =
-  exist _ (term_closure genv t) (term_closure_wf' t genv CK BC).
+  exist _ (term_closure genv t) (term_closure_wc' t genv W).
 Proof.
  apply proof_irr. cbn. now apply interp_term_carac.
 Qed.
 
-Lemma complete' A : Wf th A ->
+Lemma complete' A : WC th A ->
  IsTheorem Classic th (~A) <-> ~IsTheorem Classic th A.
 Proof.
  split.
@@ -461,85 +352,44 @@ Proof.
  - destruct (complete A); trivial. now intros [ ].
 Qed.
 
-Lemma thm_and A B :
-  IsTheorem Classic th A /\ IsTheorem Classic th B <->
-  IsTheorem Classic th (A /\ B).
-Proof.
- split.
- - intros ((WfA & axsA & FA & PRA), (WfB & axsB & FB & PRB)).
-   split. now apply Op_wf.
-   exists (axsA ++ axsB); split.
-   + rewrite Forall_forall in *; intros x; rewrite in_app_iff;
-     intros [ | ]; auto.
-   + apply R_And_i.
-     * clear PRB; eapply Pr_weakening; eauto. constructor.
-       intros a. rewrite in_app_iff; auto.
-     * eapply Pr_weakening; eauto. constructor.
-       intros a. rewrite in_app_iff; auto.
- - intros (WF & axs & F & PR); rewrite Op_wf in WF. split.
-   + split. easy.
-     exists axs; split; auto.
-     apply R_And_e1 with B; auto.
-   + split. easy.
-     exists axs; split; auto.
-     apply R_And_e2 with A; auto.
-Qed.
-
-Lemma thm_or A B : Wf th (A\/B) ->
+Lemma Thm_Or A B : WC th (A\/B) ->
   IsTheorem Classic th A \/ IsTheorem Classic th B <->
   IsTheorem Classic th (A \/ B).
 Proof.
  intros WF.
  split.
- - intros [(_ & axs & F & PR)|(_ & axs & F & PR)].
-   + split; auto. exists axs; split; auto.
-   + split; auto. exists axs; split; auto.
- - intros (_ & axs & F & PR); rewrite Op_wf in WF.
+ - now apply Thm_or_i.
+ - intros (_ & axs & F & Por); rewrite Op_WC in WF.
    destruct (complete A) as [HA|HA]; [easy|now left|].
-   destruct HA as (WfA & axsA & FA & PRA).
+   destruct HA as (_ & axsA & FA & PnA).
    destruct (complete B) as [HB|HB]; [easy|now right|].
-   destruct HB as (WfB & axsB & FB & PRB).
+   destruct HB as (_ & axsB & FB & PnB).
    destruct consistent.
-   split. apply False_wf.
-   exists (axs++axsA++axsB). split.
-   rewrite Forall_forall in *; intros x; rewrite !in_app_iff;
-     intros [|[ | ]]; auto.
+   split. apply False_WC.
+   exists (axs++axsA++axsB). split; [now rewrite !Forall_app|].
    apply R_Or_e with A B.
-   + clear PRA PRB; eapply Pr_weakening; eauto. constructor.
-     intros a. rewrite in_app_iff; auto.
-   + apply R_Not_e with A.
-     * apply R'_Ax.
-     * clear PR PRB; eapply Pr_weakening; eauto. constructor.
-       intros a. simpl. rewrite !in_app_iff; auto.
-   + apply R_Not_e with B.
-     * apply R'_Ax.
-     * clear PR PRA; eapply Pr_weakening; eauto. constructor.
-       intros a. simpl. rewrite !in_app_iff; auto.
+   + now apply Pr_app_l.
+   + eapply R_Not_e; [apply R'_Ax|].
+     now apply Pr_pop, Pr_app_r, Pr_app_l.
+   + eapply R_Not_e; [apply R'_Ax|].
+     now apply Pr_pop, Pr_app_r, Pr_app_r.
 Qed.
 
-
-Lemma thm_impl A B : Wf th (A->B) ->
+Lemma Thm_Imp A B : WC th (A->B) ->
   (IsTheorem Classic th A -> IsTheorem Classic th B) <->
   IsTheorem Classic th (A -> B).
 Proof.
- intros WF.
- split.
- - intros IM.
-   destruct (complete A) as [HA|HA]; [rewrite Op_wf in WF; easy | | ].
-   + specialize (IM HA).
-     destruct IM as (WfB & axsB & FB & PRB).
-     split; auto.
-     exists axsB; split; auto.
-     apply R_Imp_i.
-     eapply Pr_weakening; eauto. constructor. intros a; simpl; auto.
-   + destruct HA as (WfA & axsA & FA & PRA).
-     split; auto.
-     exists axsA; split; auto.
-     apply R_Imp_i.
-     apply R_Fa_e.
-     apply R_Not_e with A. apply R'_Ax.
-     eapply Pr_weakening; eauto. constructor. intros a; simpl; auto.
- - apply ModusPonens.
+ intros W. split; try apply Thm_Imp_e.
+ intros IM.
+ destruct (complete A) as [HA|HA]; [rewrite Op_WC in W; easy | | ].
+ - destruct (IM HA) as (_ & axs & F & P). split; auto.
+   exists axs; split; auto.
+   apply R_Imp_i. now apply Pr_pop.
+ - destruct HA as (_ & axs & F & P). split; auto.
+   exists axs; split; auto.
+   apply R_Imp_i.
+   apply R_Fa_e.
+   eapply R_Not_e; [apply R'_Ax|]. now apply Pr_pop.
 Qed.
 
 Lemma pr_notex_allnot logic c A :
@@ -550,15 +400,13 @@ Proof.
  - intros NE.
    apply R_All_i with x; cbn - [Names.union] in *. namedec.
    apply R_Not_i.
-   apply R_Not_e with (∃A)%form.
-   + apply R_Ex_i with (FVar x); auto using R'_Ax.
-   + eapply Pr_weakening; eauto. constructor; red; simpl; auto.
+   apply R_Not_e with (∃A)%form; [|now apply Pr_pop].
+   apply R_Ex_i with (FVar x); auto using R'_Ax.
  - intros AN.
    apply R_Not_i.
    apply R'_Ex_e with x. cbn in *. namedec.
    eapply R_Not_e; [apply R'_Ax|].
-   eapply Pr_weakening. eapply R_All_e with (t:=FVar x); eauto.
-   constructor. red; simpl; auto.
+   apply Pr_pop. now apply R_All_e with (t:=FVar x) in AN.
 Qed.
 
 Lemma pr_notexnot c A :
@@ -569,54 +417,22 @@ Proof.
  - intros NEN.
    apply R_All_i with x; cbn - [Names.union] in *. namedec.
    apply R_Absu; auto.
-   apply R_Not_e with (∃~A)%form.
+   apply R_Not_e with (∃~A)%form; [|now apply Pr_pop].
    apply R_Ex_i with (FVar x); auto using R'_Ax.
-   eapply Pr_weakening; eauto. constructor; red; simpl; auto.
  - intros ALL.
    apply R_Not_i.
-   apply R'_Ex_e with x. cbn in *. namedec.
-   cbn.
+   apply R'_Ex_e with x; cbn in *. namedec.
    eapply R_Not_e; [|eapply R'_Ax].
-   eapply Pr_weakening. eapply R_All_e with (t:=FVar x); eauto.
-   constructor. red; simpl; auto.
+   apply Pr_pop. eapply R_All_e with (t:=FVar x); eauto.
 Qed.
 
-Lemma thm_notexnot A : Wf th (∀A) ->
+Lemma thm_notexnot A : WC th (∀A) ->
   IsTheorem Classic th (~∃~A) <-> IsTheorem Classic th (∀A).
 Proof.
  intros WF.
- split; intros (_ & axs & F & P).
- - split; auto. exists axs; split; auto. now apply pr_notexnot.
- - split; auto. exists axs; split; auto. now apply pr_notexnot.
-Qed.
-
-Lemma Wf_bsubst f t :
- Wf th (∀f) -> Wf_term th t -> Wf th (bsubst 0 t f).
-Proof.
- intros (CKf & BCf & FCf) (CKt & BCt & FCt).
- repeat split.
- - apply check_bsubst; auto.
- - apply Nat.le_0_r.
-   apply level_bsubst; red in BCf; red in BCt; cbn in *; omega.
- - unfold FClosed in *. rewrite bsubst_fvars. namedec.
-Qed.
-
-Lemma thm_all_e logic A t : Wf_term th t ->
- IsTheorem logic th (∀A) -> IsTheorem logic th (bsubst 0 t A).
-Proof.
- intros WFt (WFA & axs & F & P).
- split. apply Wf_bsubst; auto.
- exists axs. split; auto.
-Qed.
-
-Lemma thm_ex_i logic A t : Wf th (∃A) ->
- IsTheorem logic th (bsubst 0 t A) ->
- IsTheorem logic th (∃A).
-Proof.
- intros WFA (_ & axs & F & P).
- split; auto.
- exists axs. split; auto.
- apply R_Ex_i with t; auto.
+ split; intros (_ & axs & F & P); split; auto; exists axs; split; auto.
+ - now apply pr_notexnot.
+ - now apply pr_notexnot.
 Qed.
 
 
@@ -647,12 +463,12 @@ Proof.
  induction h as [|h IHh]; [inversion 1|eauto].
 Qed.
 
-Lemma interp_carac f : check th f = true -> BClosed f ->
+Lemma interp_carac f : WF th f ->
  forall genv,
    interp_form mo genv [] f <->
      IsTheorem Classic th (closure genv f).
 Proof.
- induction f as [h IH f Hf] using height_ind. destruct f; intros CK BC genv.
+ induction f as [h IH f Hf] using height_ind. destruct f; intros W genv.
  - clear IH Hf. cbn.
    unfold IsTheorem. intuition.
    now exists [].
@@ -662,102 +478,84 @@ Proof.
  - clear IH Hf.
    rewrite interp_pred; auto. simpl.
    unfold vmap, vmap_list.
-   assert (forall t, In t l ->
-            proj1_sig (interp_term mo genv [] t) =
-            term_vmap (fun v : variable => proj1_sig (genv v)) t).
-   { intros t Ht. apply interp_term_carac.
-     cbn in CK.
-     destruct predsymbs; [|easy]. destruct eqb; [|easy].
-     rewrite forallb_forall in CK; auto.
-     red in BC. cbn in BC. rewrite list_max_map_0 in BC; auto. }
-   apply map_ext_iff in H. rewrite H. reflexivity.
+   f_equiv. f_equiv. apply map_ext_iff. intros t Ht.
+   apply interp_term_carac. revert t Ht. apply Forall_forall.
+   now apply Pred_WF in W.
  - simpl. rewrite IH; auto with arith.
    symmetry. apply complete'.
-   apply closure_wf; auto.
- - cbn in *. rewrite lazy_andb_iff in CK. destruct CK as (CK1,CK2).
-   red in BC. cbn in BC. apply max_0 in BC. destruct BC as (BC1,BC2).
-   destruct o; simpl; rewrite !IH; auto; try omega with *.
-   + apply thm_and.
-   + apply thm_or. apply Op_wf. split; apply (closure_wf _ genv); auto.
-   + apply thm_impl. apply Op_wf. split; apply (closure_wf _ genv); auto.
+   apply closure_wc; auto.
+ - apply Op_WF in W. cbn in Hf. apply Nat.succ_lt_mono in Hf.
+   apply max_lt in Hf.
+   destruct o; simpl; rewrite !IH by easy.
+   + apply Thm_And.
+   + apply Thm_Or. apply Op_WC. split; now apply closure_wc.
+   + apply Thm_Imp. apply Op_WC. split; now apply closure_wc.
  - simpl.
+   cbn in Hf. apply Nat.succ_lt_mono in Hf.
+   assert (L : level f <= 1).
+   { unfold WF,BClosed in W. cbn in W. omega. }
+   assert (Hf' : forall t, height (bsubst 0 t f) < h).
+   { intro. now rewrite height_bsubst. }
    destruct q; split.
    + intros H.
-     destruct (complete (closure genv (∃~f))); [apply closure_wf; auto| | ].
+     destruct (complete (closure genv (∃~f))); [apply closure_wc; auto| | ].
      * destruct (witsat (closure genv (~f)) H0) as (c & Hc & Thm).
        rewrite <- closure_bsubst in Thm by auto.
-       change (closure _ _) with (~closure genv (bsubst 0 (Cst c) f))%form in Thm.
-       assert (check th (bsubst 0 (Cst c) f) = true).
-       { apply check_bsubst; cbn; auto. now rewrite Hc, eqb_refl. }
-       assert (BClosed (bsubst 0 (Cst c) f)).
-       { apply Nat.le_0_r, level_bsubst; auto.
-         cbn. red in BC; cbn in BC. omega. }
-       rewrite complete' in Thm by (apply closure_wf; auto).
+       change (closure _ _) with (~closure genv (bsubst 0 (Cst c) f))%form
+        in Thm.
+       assert (WF th (bsubst 0 (Cst c) f)).
+       { split.
+         - apply check_bsubst; cbn; auto. now rewrite Hc, eqb_refl.
+           apply W.
+         - apply Nat.le_0_r, level_bsubst; auto. }
+       rewrite complete' in Thm by (apply closure_wc; auto).
        rewrite <- IH in Thm; auto.
-       { rewrite <- interp_form_bsubst0 in Thm; auto.
-         destruct Thm. apply H.
-         cbn. red in BC; cbn in BC. omega. }
-       { rewrite height_bsubst. cbn. cbn in Hf. omega. }
-     * apply thm_notexnot; auto.
-       apply (closure_wf (∀ f) genv); auto.
+       rewrite <- interp_form_bsubst0 in Thm; auto. destruct Thm. apply H.
+     * apply thm_notexnot; auto. apply (closure_wc (∀ f) genv); auto.
    + intros Thm (t,Ht).
-     rewrite interp_form_bsubst0 with (u:=t).
-     2:{ red in BC. cbn in BC. omega. }
-     2:{ apply Wf_term_alt in Ht. apply Ht. }
-     2:{ destruct (proj2 (Wf_term_alt _ _) Ht) as (CKt & BCt & FCt).
-         rewrite (interp_term_carac' t genv CKt BCt).
+     rewrite interp_form_bsubst0 with (u:=t); auto.
+     2:{ apply term_wc_iff in Ht. apply Ht. }
+     2:{ destruct (proj2 (term_wc_iff _ _) Ht) as (W',F').
+         rewrite (interp_term_carac' t genv W').
          apply proof_irr. cbn. apply term_vmap_id. intros v.
-         red in FCt. intuition. }
-     apply Wf_term_alt in Ht.
-     rewrite IH.
-     { rewrite closure_bsubst by apply Ht.
-       apply thm_all_e; auto. }
-     { rewrite height_bsubst. cbn in Hf. omega. }
-     { rewrite check_bsubst; auto. apply Ht. }
-     { apply Nat.le_0_r. apply level_bsubst. red in BC.
-       cbn in BC. omega. apply Nat.le_0_r, Ht. }
+         red in F'. intuition. }
+     apply term_wc_iff in Ht.
+     rewrite IH; auto.
+     * rewrite closure_bsubst by apply Ht. apply Thm_All_e; auto.
+     * apply bsubst_WF; auto. apply Ht.
    + intros ((t,Ht),Int).
-     rewrite interp_form_bsubst0 with (u:=t) in Int.
-     2:{ red in BC. cbn in BC. omega. }
+     rewrite interp_form_bsubst0 with (u:=t) in Int; auto.
+     2:{ clear Int. apply term_wc_iff in Ht. apply Ht. }
      2:{ clear Int.
-         apply Wf_term_alt in Ht. apply Ht. }
-     2:{ clear Int.
-         destruct (proj2 (Wf_term_alt _ _) Ht) as (CKt & BCt & FCt).
-         rewrite (interp_term_carac' t genv CKt BCt).
+         destruct (proj2 (term_wc_iff _ _) Ht) as (W',F').
+         rewrite (interp_term_carac' t genv W').
          apply proof_irr. cbn. apply term_vmap_id. intros v.
-         red in FCt. intuition. }
-     apply Wf_term_alt in Ht.
-     rewrite IH in Int.
-     { rewrite closure_bsubst in Int by apply Ht.
-       apply thm_ex_i with t; auto.
-       apply (closure_wf (∃f) genv); auto. }
-     { rewrite height_bsubst. cbn in Hf. omega. }
-     { rewrite check_bsubst; auto. apply Ht. }
-     { apply Nat.le_0_r. apply level_bsubst. red in BC.
-       cbn in BC. omega. apply Nat.le_0_r, Ht. }
+         red in F'. intuition. }
+     apply term_wc_iff in Ht.
+     rewrite IH in Int; auto.
+     * rewrite closure_bsubst in Int by apply Ht.
+       apply Thm_Ex_i with t; auto.
+       apply (closure_wc (∃f) genv); auto.
+     * apply bsubst_WF; auto. apply Ht.
    + intros Thm.
      destruct (witsat (closure genv f) Thm) as (c & Hc & Thm').
      rewrite <- closure_bsubst in Thm' by auto.
      rewrite <- IH in Thm'.
-     2:{ rewrite height_bsubst. cbn in Hf. omega. }
-     2:{ rewrite check_bsubst; auto. cbn. now rewrite Hc, eqb_refl. }
-     2:{ apply Nat.le_0_r. apply level_bsubst. red in BC.
-         cbn in BC. omega. auto. }
-     exists (exist _ (Cst c) (Cst_wf' th c Hc)).
+     2:{ now rewrite height_bsubst. }
+     2:{ apply bsubst_WF; auto. now apply Cst_WC. }
+     exists (exist _ (Cst c) (Cst_wc th c Hc)).
      rewrite interp_form_bsubst0; eauto.
-     { red in BC. cbn in BC. omega. }
-     { apply proof_irr. rewrite interp_term_carac; auto.
-       cbn. now rewrite Hc, eqb_refl. }
+     apply proof_irr. rewrite interp_term_carac; auto. now apply Cst_WC.
 Qed.
 
-Lemma interp_carac_closed f genv : Wf th f ->
+Lemma interp_carac_closed f genv : WC th f ->
  interp_form mo genv [] f <-> IsTheorem Classic th f.
 Proof.
- intros WF.
+ intros W.
  replace f with (closure genv f) at 2.
- apply interp_carac; apply WF.
- apply form_vmap_id. intros v. destruct WF as (_ & _ & FC).
- red in FC. intuition.
+ apply interp_carac. apply W.
+ apply form_vmap_id. intros v. destruct W as (_,F).
+ red in F. intuition.
 Qed.
 
 Lemma axioms_ok A :
@@ -765,7 +563,7 @@ Lemma axioms_ok A :
   forall genv, interp_form mo genv [] A.
 Proof.
  intros HA genv. apply interp_carac_closed.
- apply WfAxiom; auto.
+ apply WCAxiom; auto.
  apply ax_thm; auto.
 Qed.
 
@@ -844,7 +642,7 @@ Proof.
  intros CR (SE,EX) mo.
  apply Build_Model with (premodel_restrict th th' M SE mo).
  intros A HA genv.
- rewrite interp_form_restrict by (apply WfAxiom; auto).
+ rewrite interp_form_restrict by (apply WCAxiom; auto).
  assert (Thm : IsTheorem logic th' A).
  { apply EX, ax_thm; auto. }
  apply (validity_theorem logic th' CR A Thm M mo).
@@ -857,7 +655,7 @@ Lemma consistent_has_model (th:theory) (nc : NewCsts th) :
 Proof.
  intros EM C.
  set (th' := supercomplete Classic th nc).
- exists (closed_term th').
+ exists (wcterm th').
  apply (model_restrict Classic th th'). red; intros; apply EM.
  apply supercomplete_extend.
  apply SyntacticModel with (oneconst := nc 0).
@@ -877,18 +675,18 @@ Definition proj1' {A B:Prop} (c:A/\B) : A :=
 Lemma completeness_theorem (th:theory) (nc : NewCsts th) :
  (forall A, A\/~A) ->
  forall T,
-   Wf th T ->
+   WC th T ->
    (forall M (mo : Model M th) genv, interp_form mo genv [] T)
    -> IsTheorem Classic th T.
 Proof.
  intros EM T WF HT.
  destruct (EM (IsTheorem Classic th T)) as [Thm|NT]; auto.
  exfalso.
- assert (WF' : forall A, A = (~T)%form \/ IsAxiom th A -> Wf th A).
- { intros A [->|HA]; auto using WfAxiom. }
+ assert (WC' : forall A, A = (~T)%form \/ IsAxiom th A -> WC th A).
+ { intros A [->|HA]; auto using WCAxiom. }
  set (th' := {| sign := th;
                 IsAxiom := fun f => f = (~T)%form \/ IsAxiom th f;
-                WfAxiom := WF' |}).
+                WCAxiom := WC' |}).
  assert (nc' : NewCsts th').
  { apply (Build_NewCsts th')
    with (csts:=csts _ nc) (test:=test _ nc).
