Wellformed.v
@@ -1,0 +1,258 @@
+
+(** * Well-formed terms and formulas *)
+
+(** The NatDed development, Pierre Letouzey, 2019.
+    This file is released under the CC0 License, see the LICENSE file *)
+
+Require Import Defs Mix Meta.
+Local Open Scope bool_scope.
+Local Open Scope eqb_scope.
+
+(** Well-formed terms and formulas over a particular signature :
+    - use only the symbols of this signature
+    - with the correct arity
+    - and moreover with bounded variables that are indeed bounded.
+
+   Thanks to class overloading, [WF] also works for contexts, sequents,
+   derivations...
+
+   Note that a derivation which is not well-formed may still be valid
+   (in the sense of [Mix.Valid] or [Mix.Pr]). We'll see in [Restrict.v]
+   how we can force the inners of a derivation to be well-formed.
+*)
+
+Definition WF {T}`{Check T}`{Level T} sign (t:T) :=
+  check sign t = true /\ BClosed t.
+
+Definition wf {T}`{Check T}`{Level T} sign (t:T) :=
+  check sign t && (level t =? 0).
+
+(** By default, the second arguments of [WF] are to be parsed as formula. *)
+Arguments WF {T _ _} sign t%form.
+Arguments wf {T _ _} sign t%form.
+
+Lemma wf_spec {T}`{Check T}`{Level T} sign (t:T) :
+  reflect (WF sign t) (wf sign t).
+Proof.
+ unfold WF, wf, BClosed.
+ destruct check; cbn; [case eqbspec|]; now constructor.
+Qed.
+
+Lemma wf_iff {T}`{Check T}`{Level T} sign (t:T) :
+  WF sign t <-> wf sign t = true.
+Proof.
+ apply reflect_iff, wf_spec.
+Qed.
+
+Lemma Op_WF sign o A B :
+ WF sign (Op o A B) <-> WF sign A /\ WF sign B.
+Proof.
+ unfold WF, BClosed. cbn.
+ rewrite lazy_andb_iff. rewrite max_0. intuition.
+Qed.
+
+Lemma Fun_WF sign f l :
+  WF sign (Fun f l) <->
+   sign.(funsymbs) f = Some (length l) /\ Forall (WF sign) l.
+Proof.
+ unfold WF, BClosed.
+ rewrite Forall_forall. cbn.
+ destruct funsymbs as [a|]; [|easy]. rewrite lazy_andb_iff.
+ rewrite list_max_map_0, forallb_forall, eqb_eq.
+ firstorder. congruence.
+Qed.
+
+Lemma Pred_WF sign p l :
+  WF sign (Pred p l) <->
+   sign.(predsymbs) p = Some (length l) /\ Forall (WF sign) l.
+Proof.
+ unfold WF, BClosed.
+ rewrite Forall_forall. cbn.
+ destruct predsymbs as [a|]; [|easy]. rewrite lazy_andb_iff.
+ rewrite list_max_map_0, forallb_forall, eqb_eq.
+ firstorder. congruence.
+Qed.
+
+Lemma bsubst_WF sign A t :
+ WF sign (∀A) -> WF sign t -> WF sign (bsubst 0 t A).
+Proof.
+ intros (CK,BC) (CK',BC'). split.
+ - apply check_bsubst; auto.
+ - apply Nat.le_0_r.
+   apply level_bsubst; red in BC; red in BC'; cbn in *; omega.
+Qed.
+
+Lemma cons_WF sign f (c:context) :
+ WF sign (f::c) <-> WF sign f /\ WF sign c.
+Proof.
+ unfold WF, BClosed. cbn.
+ rewrite max_0, !andb_true_iff. intuition.
+Qed.
+
+Lemma ctx_WF sign (c:context) : WF sign c <-> Forall (WF sign) c.
+Proof.
+ induction c.
+ - now unfold WF, BClosed.
+ - rewrite cons_WF, IHc. split; auto.
+   now constructor. inversion 1; subst; auto.
+Qed.
+
+Lemma seq_WF sign f (c:context) :
+ WF sign (c ⊢ f) <-> WF sign c /\ WF sign f.
+Proof.
+ unfold WF, BClosed. cbn. rewrite max_0, lazy_andb_iff. intuition.
+Qed.
+
+(** WC : Well-formed Closed terms and formulas are moreover without
+    free variables. See in particular axioms and theorems in [Theory.v],
+    and points of the syntactic model in [Model.v]. *)
+
+Definition WC {T}`{Check T}`{Level T}`{FVars T} sign (t:T) :=
+  WF sign t /\ FClosed t.
+
+Definition wc {T}`{Check T}`{Level T}`{IsFClosed T} sign (t:T) :=
+  wf sign t && fclosed t.
+
+Hint Unfold WF WC.
+Arguments WC {T _ _ _} sign t%form.
+Arguments wc {T _ _ _} sign t%form.
+Implicit Types t : term.
+Implicit Types A : formula.
+
+Lemma term_wc_spec sign t : reflect (WC sign t) (wc sign t).
+Proof.
+ unfold WC, wc.
+ case wf_spec; cbn; [ | now constructor].
+ destruct (fclosed t) eqn:E.
+ - rewrite term_fclosed_spec in E. now constructor.
+ - constructor. rewrite <- term_fclosed_spec, E. easy.
+Qed.
+
+Lemma term_wc_iff sign t : WC sign t <-> wc sign t = true.
+Proof.
+ apply reflect_iff, term_wc_spec.
+Qed.
+
+Lemma wc_spec sign A : reflect (WC sign A) (wc sign A).
+Proof.
+ unfold WC, wc.
+ case wf_spec; cbn; [ | now constructor].
+ destruct (fclosed A) eqn:E.
+ - rewrite form_fclosed_spec in E. now constructor.
+ - constructor. rewrite <- form_fclosed_spec, E. easy.
+Qed.
+
+Lemma wc_iff sign A : WC sign A <-> wc sign A = true.
+Proof.
+ apply reflect_iff, wc_spec.
+Qed.
+
+Lemma WC_dec sign A : { WC sign A }+{ ~WC sign A }.
+Proof.
+ destruct (wc sign A) eqn:E; [left|right].
+ - now apply wc_iff.
+ - now rewrite wc_iff, E.
+Qed.
+
+Lemma True_WC sign : WC sign True.
+Proof.
+ now rewrite wc_iff.
+Qed.
+
+Lemma False_WC sign : WC sign False.
+Proof.
+ now rewrite wc_iff.
+Qed.
+
+Lemma Not_WC sign A : WC sign (Not A) <-> WC sign A.
+Proof.
+ now rewrite !wc_iff.
+Qed.
+
+Lemma Op_WC sign o A B :
+ WC sign (Op o A B) <-> WC sign A /\ WC sign B.
+Proof.
+ unfold WC, FClosed. cbn. rewrite Op_WF; intuition.
+Qed.
+
+Lemma bsubst_cst_WC sign c A :
+ sign.(funsymbs) c = Some 0 ->
+ WC sign (∃A) -> WC sign (bsubst 0 (Cst c) A).
+Proof.
+ intros E ((CK,BC),FC).
+ repeat split; unfold BClosed in *; cbn in *.
+ - rewrite check_bsubst; auto. cbn. now rewrite E, eqb_refl.
+ - apply Nat.le_0_r, level_bsubst; auto with *.
+ - rewrite <- !form_fclosed_spec in *. now rewrite fclosed_bsubst.
+Qed.
+
+Lemma Fun_WC sign f l :
+  WC sign (Fun f l) <->
+   sign.(funsymbs) f = Some (length l) /\ Forall (WC sign) l.
+Proof.
+ unfold WC. rewrite Fun_WF.
+ rewrite <- term_fclosed_spec. cbn.
+ rewrite forallb_forall, !Forall_forall.
+ setoid_rewrite term_fclosed_spec. intuition.
+ now apply H1. now apply H1.
+Qed.
+
+Lemma Pred_WC sign p l :
+  WC sign (Pred p l) <->
+   sign.(predsymbs) p = Some (length l) /\ Forall (WC sign) l.
+Proof.
+ unfold WC. rewrite Pred_WF.
+ rewrite <- form_fclosed_spec. cbn.
+ rewrite forallb_forall, !Forall_forall.
+ setoid_rewrite term_fclosed_spec. intuition.
+ now apply H1. now apply H1.
+Qed.
+
+Lemma Cst_WC sign c :
+  sign.(funsymbs) c = Some 0 -> WC sign (Cst c).
+Proof.
+ intros. now apply Fun_WC.
+Qed.
+
+Lemma Cst_wc sign c :
+  sign.(funsymbs) c = Some 0 -> wc sign (Cst c) = true.
+Proof.
+ rewrite <- term_wc_iff. apply Cst_WC.
+Qed.
+
+Lemma bsubst_WC sign A t :
+ WC sign (∀A) -> WC sign t -> WC sign (bsubst 0 t A).
+Proof.
+ intros (W,F) (W',F'). split.
+ - now apply bsubst_WF.
+ - rewrite <- form_fclosed_spec, fclosed_bsubst.
+   now rewrite form_fclosed_spec.
+   now rewrite term_fclosed_spec.
+Qed.
+
+Lemma WC_new_sign sign sign' A :
+ check sign' A = true -> WC sign A -> WC sign' A.
+Proof.
+ now intros ? ((?,?),?).
+Qed.
+
+Lemma cons_WC sign f (c:context) :
+ WC sign (f::c) <-> WC sign f /\ WC sign c.
+Proof.
+ unfold WC, FClosed. cbn -[Names.union].
+ rewrite cons_WF. intuition.
+Qed.
+
+Lemma ctx_WC sign (c:context) : WC sign c <-> Forall (WC sign) c.
+Proof.
+ induction c.
+ - now unfold WC, FClosed.
+ - rewrite cons_WC, IHc. split; auto.
+   now constructor. inversion 1; subst; auto.
+Qed.
+
+Lemma seq_WC sign f (c:context) :
+ WC sign (c ⊢ f) <-> WC sign c /\ WC sign f.
+Proof.
+ unfold WC, FClosed. cbn. rewrite seq_WF. intuition.
+Qed.
